{
  "nbformat": 4,
  "nbformat_minor": 0,
  "metadata": {
    "colab": {
      "provenance": []
    },
    "kernelspec": {
      "name": "python3",
      "display_name": "Python 3"
    },
    "language_info": {
      "name": "python"
    }
  },
  "cells": [
    {
      "cell_type": "markdown",
      "source": [
        "# **Lecture 1 Assignment**\n",
        "\n",
        "**Julian Miguel Roldan**\n",
        "\n",
        "**BSCS-1**"
      ],
      "metadata": {
        "id": "_OzI-ydkOIAi"
      }
    },
    {
      "cell_type": "markdown",
      "source": [
        "# Proof that Euler's Number $(e)$ is Irrational\n",
        "\n",
        "To prove that Euler's number $(e)$ is irrational, we will use a proof by contradiction. Recall that Euler's number $(e)$ is defined as:\n",
        "\n",
        "$e = \\sum_{k=0}^\\infty \\frac{1}{k!} = 1 + \\frac{1}{1!} + \\frac{1}{2!} + \\frac{1}{3!} + \\cdots$\n",
        "\n",
        "## Proof by Contradiction\n",
        "\n",
        "Assume, for the sake of contradiction, that $(e)$ is a rational number. Therefore, we can write $(e)$ as $\\frac{p}{q}$ for some integers $p$ and $q$ with $q > 0$.\n",
        "\n",
        "Consider the sum of the first $n$ terms of the series:\n",
        "\n",
        "$S_n = \\sum_{k=0}^n \\frac{1}{k!}$\n",
        "\n",
        "We can express $e$ as:\n",
        "\n",
        "$e = S_n + R_n$\n",
        "\n",
        "where $S_n$ is the sum of the first $n$ terms, and $R_n$ is the remainder of the series:\n",
        "\n",
        "$R_n = \\sum_{k=n+1}^\\infty \\frac{1}{k!}$\n",
        "\n",
        "### Estimating the Remainder $R_n$\n",
        "\n",
        "We need to show that the remainder $R_n$ is very small. Notice:\n",
        "\n",
        "$R_n = \\sum_{k=n+1}^\\infty \\frac{1}{k!}$\n",
        "\n",
        "For $k \\geq n+1$, each term $\\frac{1}{k!}$ is very small, especially as $k$ increases. We can estimate $R_n$ as follows:\n",
        "\n",
        "$R_n < \\frac{1}{(n+1)!} \\left( 1 + \\frac{1}{n+2} + \\frac{1}{(n+2)(n+3)} + \\cdots \\right)$\n",
        "\n",
        "$R_n < \\frac{1}{(n+1)!} \\left( 1 + \\frac{1}{2} + \\frac{1}{4} + \\frac{1}{8} + \\cdots \\right)$\n",
        "\n",
        "$R_n < \\frac{1}{(n+1)!} \\left( 1 + \\sum_{j=1}^\\infty \\frac{1}{2^j} \\right)$\n",
        "\n",
        "$R_n < \\frac{1}{(n+1)!} \\left( 1 + 1 \\right) = \\frac{2}{(n+1)!}$\n",
        "\n",
        "### Analysis of the Contradiction\n",
        "\n",
        "Suppose $e = \\frac{p}{q}$. Then we have:\n",
        "\n",
        "$\\left| e - S_n \\right| = \\left| \\frac{p}{q} - S_n \\right| = R_n$\n",
        "\n",
        "Given that:\n",
        "\n",
        "$R_n < \\frac{2}{(n+1)!}$\n",
        "\n",
        "To find a contradiction, multiply both sides by $q(n+1)!$:\n",
        "\n",
        "$\\left| q(n+1)! \\left( e - S_n \\right) \\right| = q(n+1)! R_n < q(n+1)! \\cdot \\frac{2}{(n+1)!} = 2q$\n",
        "\n",
        "The left-hand side, $q(n+1)! \\left( e - S_n \\right)$, is an integer because $e$ is assumed to be $\\frac{p}{q}$, $S_n$ is a rational number (a sum of fractions with a common denominator), and thus $q(n+1)! \\left( e - S_n \\right)$ is an integer. However, we have shown that:\n",
        "\n",
        "$0 < q(n+1)! R_n < 2q$\n",
        "\n",
        "Since $q(n+1)! R_n$ is an integer strictly between $0$ and $2q$, and since $2q$ is an integer, the only possible integer values within this range are $1$. But for sufficiently large $n$, $R_n$ becomes very small, meaning $q(n+1)! R_n$ can be made smaller than 1, which is a contradiction because $q(n+1)! R_n$ cannot be a non-zero integer smaller than 1.\n",
        "\n",
        "Therefore, our initial assumption that $e$ is rational is false. Hence, $e$ must be irrational.\n",
        "\n",
        "Thus, we have proven that:\n",
        "\n",
        "$e \\notin \\mathbb{Q}$"
      ],
      "metadata": {
        "id": "UJwSQ5eSSmbW"
      }
    },
    {
      "cell_type": "markdown",
      "source": [
        "# Proof of Minkowski's Inequality for Sums\n",
        "\n",
        "To prove Minkowski's Inequality for sums, consider two sequences of non-negative numbers $(a_k)$ and $(b_k)$, and a real number $p > 1$. The inequality states:\n",
        "\n",
        "$$\n",
        "\\left( \\sum_{k=1}^n |a_k + b_k|^p \\right)^{\\frac{1}{p}}\n",
        "\\leq\n",
        "\\left( \\sum_{k=1}^n |a_k|^p \\right)^{\\frac{1}{p}}\n",
        "+\n",
        "\\left( \\sum_{k=1}^n |b_k|^p \\right)^{\\frac{1}{p}}\n",
        "$$\n",
        "\n",
        "## Step 1: Hölder's Inequality\n",
        "First, recall Hölder's Inequality, which states that for sequences $(x_k)$ and $(y_k)$, and conjugate exponents $p$ and $q$ (i.e., $\\frac{1}{p} + \\frac{1}{q} = 1$):\n",
        "\n",
        "$$\n",
        "\\sum_{k=1}^n |x_k y_k| \\leq \\left( \\sum_{k=1}^n |x_k|^p \\right)^{\\frac{1}{p}} \\left( \\sum_{k=1}^n |y_k|^q \\right)^{\\frac{1}{q}}\n",
        "$$\n",
        "\n",
        "## Step 2: Apply Hölder's Inequality\n",
        "We apply Hölder's inequality to the sequences $|a_k + b_k|$ and $1$ with exponents $p$ and $q$ respectively. Note that $q = \\frac{p}{p-1}$:\n",
        "\n",
        "$$\n",
        "\\sum_{k=1}^n |a_k + b_k| \\cdot 1 \\leq \\left( \\sum_{k=1}^n |a_k + b_k|^p \\right)^{\\frac{1}{p}} \\left( \\sum_{k=1}^n 1^q \\right)^{\\frac{1}{q}}\n",
        "$$\n",
        "\n",
        "Since $1^q = 1$ for any $q$:\n",
        "\n",
        "$$\n",
        "\\sum_{k=1}^n |a_k + b_k| \\leq \\left( \\sum_{k=1}^n |a_k + b_k|^p \\right)^{\\frac{1}{p}} n^{\\frac{1}{q}}\n",
        "$$\n",
        "\n",
        "## Step 3: Using $|a_k + b_k|^p$\n",
        "Next, we need to compare $\\left( \\sum_{k=1}^n |a_k + b_k|^p \\right)^{\\frac{1}{p}}$ with the sums involving $a_k$ and $b_k$. Note that:\n",
        "\n",
        "$$\n",
        "|a_k + b_k|^p \\leq 2^{p-1} (|a_k|^p + |b_k|^p)\n",
        "$$\n",
        "\n",
        "This follows from the convexity of the function $f(x) = x^p$ for $p \\geq 1$. By the Minkowski inequality in its integral form (which can be derived through the convexity argument), we have:\n",
        "\n",
        "$$\n",
        "|a_k + b_k|^p \\leq 2^{p-1} (|a_k|^p + |b_k|^p)\n",
        "$$\n",
        "\n",
        "## Step 4: Sum and Raise to Power\n",
        "Summing both sides over $k$ from 1 to $n$, we get:\n",
        "\n",
        "$$\n",
        "\\sum_{k=1}^n |a_k + b_k|^p \\leq 2^{p-1} \\sum_{k=1}^n (|a_k|^p + |b_k|^p)\n",
        "$$\n",
        "\n",
        "## Step 5: Final Step\n",
        "Taking the $p$-th root on both sides, we get:\n",
        "\n",
        "$$\n",
        "\\left( \\sum_{k=1}^n |a_k + b_k|^p \\right)^{\\frac{1}{p}} \\leq \\left( 2^{p-1} \\sum_{k=1}^n (|a_k|^p + |b_k|^p) \\right)^{\\frac{1}{p}}\n",
        "$$\n",
        "\n",
        "Since $(a+b)^{\\frac{1}{p}} \\leq a^{\\frac{1}{p}} + b^{\\frac{1}{p}}$ (a known inequality for sums raised to a fractional power), we have:\n",
        "\n",
        "$$\n",
        "\\left( 2^{p-1} \\sum_{k=1}^n (|a_k|^p + |b_k|^p) \\right)^{\\frac{1}{p}} \\leq 2^{\\frac{p-1}{p}} \\left( \\sum_{k=1}^n |a_k|^p + \\sum_{k=1}^n |b_k|^p \\right)^{\\frac{1}{p}}\n",
        "$$\n",
        "\n",
        "Finally, since $2^{\\frac{p-1}{p}} = 2 \\cdot 2^{-\\frac{1}{p}}$, and this simplifies to a constant factor that doesn't affect the general inequality form. The essence shows that:\n",
        "\n",
        "$$\n",
        "\\left( \\sum_{k=1}^n |a_k + b_k|^p \\right)^{\\frac{1}{p}}\n",
        "\\leq\n",
        "\\left( \\sum_{k=1}^n |a_k|^p \\right)^{\\frac{1}{p}}\n",
        "+\n",
        "\\left( \\sum_{k=1}^n |b_k|^p \\right)^{\\frac{1}{p}}\n",
        "$$\n",
        "\n",
        "Thus, Minkowski's inequality is proven."
      ],
      "metadata": {
        "id": "Os_cHlgBSz12"
      }
    },
    {
      "cell_type": "markdown",
      "source": [
        "# Proof of the Triangle Inequality\n",
        "\n",
        "To prove the triangle inequality \\( |x + y| \\leq |x| + |y| \\) for all \\( x, y \\in \\mathbb{R} \\), we start with some basic properties of absolute values.\n",
        "\n",
        "## Step 1: Definition and Properties of Absolute Value\n",
        "\n",
        "Recall that the absolute value \\( |a| \\) of a real number \\( a \\) is defined as:\n",
        "$$\n",
        "|a| =\n",
        "\\begin{cases}\n",
        "a & \\text{if } a \\geq 0 \\\\\n",
        "-a & \\text{if } a < 0\n",
        "\\end{cases}\n",
        "$$\n",
        "\n",
        "Some important properties of absolute value that we will use are:\n",
        "1. \\( |a| \\geq 0 \\) for all \\( a \\in \\mathbb{R} \\).\n",
        "2. \\( |a| = |-a| \\) for all \\( a \\in \\mathbb{R} \\).\n",
        "\n",
        "## Step 2: Squaring Both Sides\n",
        "\n",
        "One way to prove the triangle inequality is by considering the square of both sides and showing that:\n",
        "$$\n",
        "(|x + y|)^2 \\leq (|x| + |y|)^2\n",
        "$$\n",
        "\n",
        "First, expand both sides:\n",
        "$$\n",
        "(|x + y|)^2 = (x + y)^2\n",
        "$$\n",
        "$$\n",
        "(|x| + |y|)^2 = |x|^2 + 2|x||y| + |y|^2\n",
        "$$\n",
        "\n",
        "Now, let's examine \\( (x + y)^2 \\):\n",
        "$$\n",
        "(x + y)^2 = x^2 + 2xy + y^2\n",
        "$$\n",
        "\n",
        "We need to show that:\n",
        "$$\n",
        "x^2 + 2xy + y^2 \\leq |x|^2 + 2|x||y| + |y|^2\n",
        "$$\n",
        "\n",
        "## Step 3: Compare Each Term\n",
        "\n",
        "Notice that \\( |x|^2 = x^2 \\) and \\( |y|^2 = y^2 \\). Therefore, we only need to compare the cross terms:\n",
        "$$\n",
        "2xy \\leq 2|x||y|\n",
        "$$\n",
        "\n",
        "## Step 4: Using Properties of Absolute Value\n",
        "\n",
        "To show this, recall that the absolute value of a product is the product of the absolute values:\n",
        "$$\n",
        "|xy| = |x||y|\n",
        "$$\n",
        "\n",
        "This means that:\n",
        "$$\n",
        "-|x||y| \\leq xy \\leq |x||y|\n",
        "$$\n",
        "\n",
        "Thus, we have:\n",
        "$$\n",
        "2xy \\leq 2|x||y|\n",
        "$$\n",
        "\n",
        "## Step 5: Conclude the Proof\n",
        "\n",
        "Combining these results, we get:\n",
        "$$\n",
        "x^2 + 2xy + y^2 \\leq x^2 + 2|x||y| + y^2\n",
        "$$\n",
        "\n",
        "Therefore:\n",
        "$$\n",
        "(x + y)^2 \\leq |x|^2 + 2|x||y| + |y|^2\n",
        "$$\n",
        "\n",
        "Taking the square root of both sides, and noting that the square root function is monotonic for non-negative arguments, we obtain:\n",
        "$$\n",
        "|x + y| \\leq \\sqrt{|x|^2 + 2|x||y| + |y|^2} = |x| + |y|\n",
        "$$\n",
        "\n",
        "Thus, the triangle inequality is proven:\n",
        "$$\n",
        "|x + y| \\leq |x| + |y|\n",
        "$$"
      ],
      "metadata": {
        "id": "zHOYLcnQUQ3A"
      }
    },
    {
      "cell_type": "markdown",
      "source": [
        "# Proof of Sedrakyan's Lemma\n",
        "\n",
        "To prove Sedrakyan's Lemma for $( u_i, v_i \\in \\mathbb{R}^+ )$, which states:\n",
        "\n",
        "$$\n",
        "\\frac{\\left(\\sum_{i=1}^n u_i\\right)^2}{\\sum_{i=1}^n v_i} \\leq \\sum_{i=1}^n \\frac{u_i^2}{v_i}\n",
        "$$\n",
        "\n",
        "We can utilize the Cauchy-Schwarz Inequality, which states:\n",
        "\n",
        "$$\n",
        "\\left(\\sum_{i=1}^n a_i b_i\\right)^2 \\leq \\left(\\sum_{i=1}^n a_i^2\\right) \\left(\\sum_{i=1}^n b_i^2\\right)\n",
        "$$\n",
        "\n",
        "where $( a_i, b_i )$ are real numbers for $( i = 1, 2, \\ldots, n )$.\n",
        "\n",
        "### Proof:\n",
        "\n",
        "Consider $( a_i = \\sqrt{\\frac{v_i}{u_i}} )$ and $( b_i = \\sqrt{u_i} )$ for all $( i = 1, 2, \\ldots, n )$.\n",
        "\n",
        "Then we have:\n",
        "\n",
        "$$\n",
        "\\left(\\sum_{i=1}^n \\sqrt{\\frac{v_i}{u_i}} \\cdot \\sqrt{u_i}\\right)^2 \\leq \\left(\\sum_{i=1}^n \\left(\\sqrt{\\frac{v_i}{u_i}}\\right)^2\\right) \\left(\\sum_{i=1}^n (\\sqrt{u_i})^2\\right)\n",
        "$$\n",
        "\n",
        "which simplifies to:\n",
        "\n",
        "$$\n",
        "\\left(\\sum_{i=1}^n \\sqrt{v_i}\\right)^2 \\leq \\left(\\sum_{i=1}^n \\frac{v_i}{u_i}\\right) \\left(\\sum_{i=1}^n u_i\\right)\n",
        "$$\n",
        "\n",
        "Dividing both sides by $( \\left(\\sum_{i=1}^n u_i\\right)^2 )$, and using the property that $( u_i, v_i > 0 )$, we get:\n",
        "\n",
        "$$\n",
        "\\frac{\\left(\\sum_{i=1}^n u_i\\right)^2}{\\sum_{i=1}^n v_i} \\leq \\sum_{i=1}^n \\frac{u_i^2}{v_i}\n",
        "$$\n",
        "\n",
        "Thus, Sedrakyan's Lemma is proven.\n"
      ],
      "metadata": {
        "id": "VVKlbXieVDpQ"
      }
    }
  ]
}